Checkin before linearity checks

reduce/WorkStealing.v
@@ -1,17 +1,5 @@
 Require Export ProcessRewrite.
 Require Export RewriteTactics.
-(** 
-< q             ▹ foreach (i ∈ [1..n]):
-                                 ∀p. recv(p); send(p, Integer);
-                               μX. ∀p. recv(p); send(p, tt); X
-               p[len slaves] ▹ μX. send(q, me); { recv(Int); send(me, Int); X
-                                                , recv(tt)
-                                                };
-               me            ▹ foreach (i ∈ [1..n]):
-                                 recv(Integer)
-             > Integer
-**)
-
 
 Inductive Message :=
   | int
@@ -50,3 +38,62 @@ Proof.
   apply stmt_fold_loop.
   skip.
 Qed.
+
+Definition sendn {T:Type} p m := @s_send T p (m, p_none).
+Definition recvn {T:Type} m := @s_recv T (m, p_none).
+
+Example choice0 :
+  [ q [[ s_iter xs (sendn (p_sng me) int; sendn (p_sng me) tt) ]]
+  | me[[ s_iter xs (s_ext_ch (recvn int) (recvn tt);
+                    s_ext_ch (recvn int) (recvn tt)) ]]
+  ] ===>
+  [ q [[ s_skip ]] 
+  | me[[ s_skip ]]
+  ].
+Proof.
+  choose_left 1.
+  reduce_pair 0 1.
+  choose_right 1.
+  reduce_pair 0 1.
+  skip.
+Qed.
+
+(** 
+< q             ▹ foreach (i ∈ [1..n]):
+                                 ∀p. recv(p); send(p, Integer);
+                               μX. ∀p. recv(p); send(p, tt); X
+               p[len slaves] ▹ μX. send(q, me); { recv(Int); send(me, Int); X
+                                                , recv(tt)
+                                                };
+               me            ▹ foreach (i ∈ [1..n]):
+                                 recv(Integer)
+             > Integer
+**)
+
+(** Wait how come this works? What if the last line was 1..n+1? **)
+(** I think the answer is that the "context" is the product of the number
+    of grouped process and the loop, thus the loop is unrolled Y times 
+    such that len slaves * Y = n. So a loop unrolling must be rewritten
+    into an iter before progress can be made **)
+
+Example WorkStealing :
+  [ q   [[ s_iter xs (x ~ (s_recv (id, p_sng x);
+                         s_send (p_sng x) (int, p_none)));
+           s_loop X (x ~ (s_recv (id, p_sng x);
+                          s_send (p_sng x) (tt, p_none);
+                          s_var X)) ]]
+  |{ps} [[ s_loop X (s_send (p_sng q) (id, p_set ps);
+                     s_ext_ch (s_recv (int, p_none); s_send (p_sng me) (int, p_none); s_var X)
+                              (s_recv (tt, p_none))) ]]
+  | me  [[ s_iter xs (s_recv (int, p_none)) ]] ] ===>
+ [ q [[ s_skip ]] | { ps } [[ s_skip ]] | me [[ s_skip ]] ].
+Proof.
+  inst_bind 0.
+  rewrite_eq_stmt 1.
+  apply stmt_unfold_loop.
+  reduce_pair 0 1.
+  choose_left 1.
+  reduce_pair 0 1.
+  reduce_pair 1 2.
+  rewrite_eq_stmt 1.
+  apply stmt_fold_loop.
