reduce/LoopTest.v
@@ -1,0 +1,30 @@
+Require Export ProcessRewrite.
+Require Export RewriteTactics.
+
+Example SillyLoop :
+  forall (p q : nat) (x : MuVar) (ps : SetVar),
+    [ p [[ s_loop x (s_send (p_sng q) (tt, p_none); s_var x) ]] 
+    | q [[ s_loop x (s_recv (tt, p_none); s_var x) ]] ]
+    ===> [ { ps } [[ s_skip ]] | q [[ s_skip ]] ].
+Proof.
+  intros.
+  eapply rewrite_trans; 
+    [ eapply rewrite_unroll_loop with (i := 0); simpl | idtac]. 
+  reflexivity.
+  reflexivity.
+  simpl.
+  eapply rewrite_trans; 
+    [ eapply rewrite_unroll_loop with (i := 1); simpl | idtac]. 
+  reflexivity.
+  reflexivity.
+  simpl.
+  reduce_pair 0 1.
+  eapply rewrite_trans.
+  eapply rewrite_elim_unroll with (i := 0).
+  cbv. reflexivity.
+  cbv. reflexivity.
+  cbv. reflexivity.
+  cbv.
+  apply rewrite_pair with (i1 := 0) (i2 := 1).
+  reflexivity.
+  reflexivity.
