reduce/MasterSlave.v
@@ -1,0 +1,23 @@
+Require Export ProcessRewrite.
+Require Export RewriteTactics.
+
+Inductive Message :=
+  | Integer.
+
+Example MasterSlave :
+  forall (p : pid) (xs : SetVar) (qs : SetVar),
+    measure xs = measure qs ->
+    [ p    [[ s_iter xs (s_recv (Integer, p_none)) ]]
+    | {qs} [[ s_send (p_sng p) (Integer, p_none) ]]
+    ] 
+      ===> 
+    [ p    [[ s_skip ]]
+    | {qs} [[ s_skip ]]
+    ].
+Proof.
+  intros.
+  rewrite_eq_stmt 0.
+  apply stmt_set; auto.
+  reduce_pair 0 1.
+  skip.
+Qed.
