reduce/RewriteTactics.v
@@ -1,9 +1,13 @@
 Require Export ProcessRewrite.
 
+Hint Constructors EqStmt : eqstmt.
+
 Ltac skip := solve[apply rewrite_refl].
 
-Ltac apply_rewrite x :=
-  eapply rewrite_trans; [ x | idtac].
+Ltac rewrite_eq_stmt x :=
+  eapply rewrite_trans; 
+  [ eapply rewrite_eq_stmt with (i := x ); cbv; try reflexivity | idtac]; 
+  try reflexivity; cbv.
 
 Ltac reduce_pair i j :=
   eapply rewrite_trans;
@@ -18,7 +22,17 @@ Ltac expand_subst :=
                destruct (eq_dec_pid x y); [ congruence | idtac]
            end.
 
-Ltac inst_bind i x :=
+Ltac inst_bind x :=
   eapply rewrite_trans; [
-    eapply rewrite_bind with (1 := i) (3 := x); simpl; try reflexivity
-    | expand_subst].
+      eapply rewrite_bind with (i := x)
+    | idtac ]; simpl; try reflexivity; expand_subst.
+
+Ltac choose_left x :=
+  eapply rewrite_trans; 
+  [ eapply rewrite_ext_choice_l with (i := x); try reflexivity | idtac];
+  simpl. 
+
+Ltac choose_right x :=
+  eapply rewrite_trans; 
+  [ eapply rewrite_ext_choice_r with (i := x); try reflexivity | idtac];
+  simpl. 
